global ioa specification.

Isabelle2/AbstractMultiPaxosR3.thy
@@ -1,7 +1,7 @@
 chapter {* Distributed and executable algorithm *}
 
 theory AbstractMultiPaxosR3 
-  imports Utils "~~/src/HOL/Library/FinFun" MaxByKey IOA
+  imports Utils "~~/src/HOL/Library/FinFun" MaxByKey IOA Quorums
 begin
 
 unbundle finfun_syntax
@@ -16,6 +16,7 @@ subsection {* Data structures *}
 locale amp_r3 =
   fixes leader :: "bal \<Rightarrow> 'a::linorder"
   and next_bal :: "bal \<Rightarrow> 'a \<Rightarrow> bal"
+  and as :: "'a set"
   and quorums :: "'a set set"
 begin
   
@@ -54,7 +55,7 @@ datatype ('aa,'vv) msg =
 datatype ('aa,'vv) packet =
   Packet 'aa  "('aa,'vv) msg"
 
-definition local_start where "local_start a as \<equiv>
+definition local_start where "local_start a \<equiv>
   \<lparr>id = a, acceptors = as, ballot = 0, log = K$ Free,
     votes = K$ None, onebs = K$ None, twobs = K$ K$ {}\<rparr>"
 
@@ -258,8 +259,8 @@ record ('a,'v) global_state =
 
 context amp_r3 begin
 
-definition global_start where "global_start as \<equiv>
-  \<lparr>local_states = (\<lambda> a . local_start a as), network = {}\<rparr>"
+definition global_start where "global_start \<equiv>
+  \<lparr>local_states = (\<lambda> a . local_start a), network = {}\<rparr>"
 
 inductive_set trans_rel :: "(('a,'v) global_state \<times> 'v action \<times> ('a,'v) global_state) set" where
   "\<lbrakk>(Packet a m) \<in> network s; process_msg ((local_states s) a) m = (sa', ms); m = Phase2b a i b v;
@@ -276,17 +277,42 @@ inductive_set trans_rel :: "(('a,'v) global_state \<times> 'v action \<times> ('
     \<Longrightarrow> (s, Propose v, 
       s\<lparr>local_states := (local_states s)(a := sa'), network := network s \<union> ms\<rparr>) \<in> trans_rel"
 
-end 
+end
+
+definition n :: nat where "n \<equiv> 3"
+  -- {* The number of processes *}
+
+definition accs where "accs \<equiv> {1..n}"
+  -- {* The set of acceptors *}
+
+definition leader where "leader (b::nat) \<equiv> (b mod n) + 1"
+  
+definition next_bal :: "nat \<Rightarrow> nat \<Rightarrow> nat" where "next_bal b a \<equiv> 
+  (b div n + 1) * n + a"
+  
+global_interpretation cq:card_quorums accs
+  defines qs = "cq.quorums" and nas = "cq.nas"
+  apply (unfold_locales)
+   apply (simp add: accs_def n_def)
+  apply (simp add: accs_def)
+  done
+
+global_interpretation my_amp_r3:amp_r3 leader next_bal accs qs 
+  defines start = my_amp_r3.global_start
+    and trans = my_amp_r3.trans_rel
+    and propose = my_amp_r3.propose
+    and try_acquire_leadership = my_amp_r3.try_acquire_leadership
+    and process_msg = my_amp_r3.process_msg
+    and local_start = my_amp_r3.local_start
+    and receive_fwd = my_amp_r3.receive_fwd
+    and receive_1a = my_amp_r3.receive_1a
+  .
+
+definition ioa where
+  "ioa \<equiv> \<lparr>ioa.asig = amp_r3.asig, ioa.start = {start}, ioa.trans = trans\<rparr>"
 
 subsection {* Code generation *}
 
-global_interpretation ldefs:amp_r3 leader next_bal quorums for leader next_bal quorums 
-  defines propose = amp_r3.propose
-    and try_acquire_leadership = amp_r3.try_acquire_leadership
-    and process_msg = amp_r3.process_msg
-    and start = amp_r3.local_start
-  .
-
-export_code start propose try_acquire_leadership process_msg in Scala
+export_code local_start propose try_acquire_leadership process_msg in Scala
 
 end
